PREFIX cpm:    <http://purl.org/voc/cpm#>
PREFIX dc:     <http://purl.org/dc/terms/>
PREFIX dcat:   <http://www.w3.org/ns/dcat#>
PREFIX dce:    <http://purl.org/dc/elements/1.1/>
PREFIX dct:    <http://purl.org/dc/terms/>
PREFIX grg:    <http://www.isotc211.org/schemas/grg/>
PREFIX iop:    <https://w3id.org/iadopt/ont#>
PREFIX ns0:    <http://www.w3.org/ns/dx/conneg/altr#>
PREFIX ns1:    <http://www.w3.org/ns/dx/prof/>
PREFIX owl:    <http://www.w3.org/2002/07/owl#>
PREFIX pav:    <http://purl.org/pav/>
PREFIX prov:   <https://www.w3.org/ns/prov#>
PREFIX puv:    <https://w3id.org/env/puv#>
PREFIX qudt:   <https://qudt.org/2.1/schema/qudt#>
PREFIX rdf:    <http://www.w3.org/1999/02/22-rdf-syntax-ns#>
PREFIX rdfs:   <http://www.w3.org/2000/01/rdf-schema#>
PREFIX reg:    <http://purl.org/linked-data/registry#>
PREFIX semapv: <http://w3id.org/semapv/vocab/>
PREFIX skos:   <http://www.w3.org/2004/02/skos/core#>
PREFIX sssom:  <https://w3id.org/sssom/schema/>
PREFIX void:   <http://rdfs.org/ns/void#>

<http://vocab.nerc.ac.uk/collection/C34/current/MRAT0014/>
        rdf:type               skos:Concept;
        dce:identifier         "SDN:C34::MRAT0014";
        dc:date                "2007-06-29 16:19:24.0";
        dc:identifier          "SDN:C34::MRAT0014";
        pav:authoredOn         "2007-06-29 16:19:24.0";
        pav:hasCurrentVersion  <http://vocab.nerc.ac.uk/collection/C34/current/MRAT0014/1/>;
        pav:version            "1";
        void:inDataset         <http://vocab.nerc.ac.uk/.well-known/void>;
        owl:deprecated         "false";
        owl:versionInfo        "1";
        skos:altLabel          "Litter";
        skos:definition        "The degradation of the environment from waste types consisting of any tangible personal property which has been unlawfully scattered and or abandoned"@en;
        skos:notation          "SDN:C34::MRAT0014";
        skos:note              "accepted"@en;
        skos:prefLabel         "Litter"@en .

<http://vocab.nerc.ac.uk/collection/C34/current/MRAT0022/>
        rdf:type               skos:Concept;
        dce:identifier         "SDN:C34::MRAT0022";
        dc:date                "2011-02-24 15:47:45.0";
        dc:identifier          "SDN:C34::MRAT0022";
        pav:authoredOn         "2011-02-24 15:47:45.0";
        pav:hasCurrentVersion  <http://vocab.nerc.ac.uk/collection/C34/current/MRAT0022/1/>;
        pav:version            "1";
        void:inDataset         <http://vocab.nerc.ac.uk/.well-known/void>;
        owl:deprecated         "false";
        owl:versionInfo        "1";
        skos:altLabel          "Operational oceanography";
        skos:definition        "Monitoring activities that are carried out to provide oceanographic forecasts and services to the public and scientific community. They do not provide information on a specific environmental pressure."@en;
        skos:notation          "SDN:C34::MRAT0022";
        skos:note              "accepted"@en;
        skos:prefLabel         "Operational oceanography"@en .

<http://vocab.nerc.ac.uk/collection/C34/current/MRAT0002/>
        rdf:type               skos:Concept;
        dce:identifier         "SDN:C34::MRAT0002";
        dc:date                "2007-06-29 16:19:24.0";
        dc:identifier          "SDN:C34::MRAT0002";
        pav:authoredOn         "2007-06-29 16:19:24.0";
        pav:hasCurrentVersion  <http://vocab.nerc.ac.uk/collection/C34/current/MRAT0002/1/>;
        pav:version            "1";
        void:inDataset         <http://vocab.nerc.ac.uk/.well-known/void>;
        owl:deprecated         "false";
        owl:versionInfo        "1";
        skos:altLabel          "Shoreline reinforcement";
        skos:definition        "Alteration of the coastline for the protection of land from the sea"@en;
        skos:notation          "SDN:C34::MRAT0002";
        skos:note              "accepted"@en;
        skos:prefLabel         "Shoreline reinforcement"@en .

<http://vocab.nerc.ac.uk/collection/C34/current/MRAT0007/>
        rdf:type               skos:Concept;
        dce:identifier         "SDN:C34::MRAT0007";
        dc:date                "2007-12-05 16:09:24.0";
        dc:identifier          "SDN:C34::MRAT0007";
        pav:authoredOn         "2007-12-05 16:09:24.0";
        pav:hasCurrentVersion  <http://vocab.nerc.ac.uk/collection/C34/current/MRAT0007/2/>;
        pav:hasVersion         <http://vocab.nerc.ac.uk/collection/C34/current/MRAT0007/1/>;
        pav:version            "2";
        void:inDataset         <http://vocab.nerc.ac.uk/.well-known/void>;
        owl:deprecated         "false";
        owl:versionInfo        "2";
        skos:altLabel          "Commercial fishing";
        skos:definition        "The removal of wild fish from the environment by humans"@en;
        skos:notation          "SDN:C34::MRAT0007";
        skos:note              "accepted"@en;
        skos:prefLabel         "Commercial fishing"@en .

<http://vocab.nerc.ac.uk/collection/C34/current/MRAT0017/>
        rdf:type               skos:Concept;
        dce:identifier         "SDN:C34::MRAT0017";
        dc:date                "2007-12-05 15:59:02.0";
        dc:identifier          "SDN:C34::MRAT0017";
        pav:authoredOn         "2007-12-05 15:59:02.0";
        pav:hasCurrentVersion  <http://vocab.nerc.ac.uk/collection/C34/current/MRAT0017/1/>;
        pav:version            "1";
        void:inDataset         <http://vocab.nerc.ac.uk/.well-known/void>;
        owl:deprecated         "false";
        owl:versionInfo        "1";
        skos:altLabel          "Coastal and offshore infrastructure";
        skos:definition        "Physical effects on the water column or seabed caused by coastal and offshore infrastructure (eg marinas, harbours, oil and gas platforms, wind turbines)"@en;
        skos:notation          "SDN:C34::MRAT0017";
        skos:note              "accepted"@en;
        skos:prefLabel         "Coastal and offshore infrastructure"@en .

<http://vocab.nerc.ac.uk/collection/C34/current/MRAT0004/>
        rdf:type               skos:Concept;
        dce:identifier         "SDN:C34::MRAT0004";
        dc:date                "2007-06-29 16:19:24.0";
        dc:identifier          "SDN:C34::MRAT0004";
        pav:authoredOn         "2007-06-29 16:19:24.0";
        pav:hasCurrentVersion  <http://vocab.nerc.ac.uk/collection/C34/current/MRAT0004/1/>;
        pav:version            "1";
        void:inDataset         <http://vocab.nerc.ac.uk/.well-known/void>;
        owl:deprecated         "false";
        owl:versionInfo        "1";
        skos:altLabel          "Dredge disposal";
        skos:definition        "The disposal of material which originates from the seabed"@en;
        skos:notation          "SDN:C34::MRAT0004";
        skos:note              "accepted"@en;
        skos:prefLabel         "Dredge disposal"@en .

<http://vocab.nerc.ac.uk/collection/C34/current/MRAT0018/>
        rdf:type               skos:Concept;
        dce:identifier         "SDN:C34::MRAT0018";
        dc:date                "2007-12-05 16:02:16.0";
        dc:identifier          "SDN:C34::MRAT0018";
        pav:authoredOn         "2007-12-05 16:02:16.0";
        pav:hasCurrentVersion  <http://vocab.nerc.ac.uk/collection/C34/current/MRAT0018/1/>;
        pav:version            "1";
        void:inDataset         <http://vocab.nerc.ac.uk/.well-known/void>;
        owl:deprecated         "false";
        owl:versionInfo        "1";
        skos:altLabel          "Noise";
        skos:definition        "The introduction of noise into the marine environment such as by siesmic surveys, shipping or coastal and offshore infrastructure."@en;
        skos:notation          "SDN:C34::MRAT0018";
        skos:note              "accepted"@en;
        skos:prefLabel         "Noise"@en .

<http://vocab.nerc.ac.uk/collection/C34/current/MRAT0005/>
        rdf:type               skos:Concept;
        dce:identifier         "SDN:C34::MRAT0005";
        dc:date                "2007-06-29 16:19:24.0";
        dc:identifier          "SDN:C34::MRAT0005";
        pav:authoredOn         "2007-06-29 16:19:24.0";
        pav:hasCurrentVersion  <http://vocab.nerc.ac.uk/collection/C34/current/MRAT0005/1/>;
        pav:version            "1";
        void:inDataset         <http://vocab.nerc.ac.uk/.well-known/void>;
        owl:deprecated         "false";
        owl:versionInfo        "1";
        skos:altLabel          "Aggregate extraction";
        skos:definition        "The extraction of material from the seabed for economic profit"@en;
        skos:notation          "SDN:C34::MRAT0005";
        skos:note              "accepted"@en;
        skos:prefLabel         "Aggregate extraction"@en .

<http://vocab.nerc.ac.uk/collection/C34/current/MRAT0015/>
        rdf:type               skos:Concept;
        dce:identifier         "SDN:C34::MRAT0015";
        dc:date                "2007-06-29 16:19:24.0";
        dc:identifier          "SDN:C34::MRAT0015";
        pav:authoredOn         "2007-06-29 16:19:24.0";
        pav:hasCurrentVersion  <http://vocab.nerc.ac.uk/collection/C34/current/MRAT0015/1/>;
        pav:version            "1";
        void:inDataset         <http://vocab.nerc.ac.uk/.well-known/void>;
        owl:deprecated         "false";
        owl:versionInfo        "1";
        skos:altLabel          "Unknown";
        skos:definition        "The correct value is not known to, and not computable by, the sender of this data. However, a correct value probably exists"@en;
        skos:notation          "SDN:C34::MRAT0015";
        skos:note              "accepted"@en;
        skos:prefLabel         "Unknown"@en .

<http://vocab.nerc.ac.uk/collection/C34/current/MRAT0003/>
        rdf:type               skos:Concept;
        dce:identifier         "SDN:C34::MRAT0003";
        dc:date                "2007-06-29 16:19:24.0";
        dc:identifier          "SDN:C34::MRAT0003";
        pav:authoredOn         "2007-06-29 16:19:24.0";
        pav:hasCurrentVersion  <http://vocab.nerc.ac.uk/collection/C34/current/MRAT0003/1/>;
        pav:version            "1";
        void:inDataset         <http://vocab.nerc.ac.uk/.well-known/void>;
        owl:deprecated         "false";
        owl:versionInfo        "1";
        skos:altLabel          "Dredging";
        skos:definition        "The removal of material from the seabed"@en;
        skos:notation          "SDN:C34::MRAT0003";
        skos:note              "accepted"@en;
        skos:prefLabel         "Dredging"@en .

<http://vocab.nerc.ac.uk/collection/C34/current/MRAT0019/>
        rdf:type               skos:Concept;
        dce:identifier         "SDN:C34::MRAT0019";
        dc:date                "2007-12-05 16:03:21.0";
        dc:identifier          "SDN:C34::MRAT0019";
        pav:authoredOn         "2007-12-05 16:03:21.0";
        pav:hasCurrentVersion  <http://vocab.nerc.ac.uk/collection/C34/current/MRAT0019/1/>;
        pav:version            "1";
        void:inDataset         <http://vocab.nerc.ac.uk/.well-known/void>;
        owl:deprecated         "false";
        owl:versionInfo        "1";
        skos:altLabel          "Temperature modification";
        skos:definition        "Localised temperature changes caused by human activities such as power stations."@en;
        skos:notation          "SDN:C34::MRAT0019";
        skos:note              "accepted"@en;
        skos:prefLabel         "Temperature modification"@en .

<http://vocab.nerc.ac.uk/collection/C34/current/MRAT0010/>
        rdf:type               skos:Concept;
        dce:identifier         "SDN:C34::MRAT0010";
        dc:date                "2007-06-29 16:19:24.0";
        dc:identifier          "SDN:C34::MRAT0010";
        pav:authoredOn         "2007-06-29 16:19:24.0";
        pav:hasCurrentVersion  <http://vocab.nerc.ac.uk/collection/C34/current/MRAT0010/1/>;
        pav:version            "1";
        void:inDataset         <http://vocab.nerc.ac.uk/.well-known/void>;
        owl:deprecated         "false";
        owl:versionInfo        "1";
        skos:altLabel          "Hazardous substances enrichment";
        skos:definition        "The enrichment of chemicals that are potentially toxic above natural levels"@en;
        skos:notation          "SDN:C34::MRAT0010";
        skos:note              "accepted"@en;
        skos:prefLabel         "Hazardous substances enrichment"@en .

<http://vocab.nerc.ac.uk/collection/C34/current/MRAT0013/>
        rdf:type               skos:Concept;
        dce:identifier         "SDN:C34::MRAT0013";
        dc:date                "2007-06-29 16:19:24.0";
        dc:identifier          "SDN:C34::MRAT0013";
        pav:authoredOn         "2007-06-29 16:19:24.0";
        pav:hasCurrentVersion  <http://vocab.nerc.ac.uk/collection/C34/current/MRAT0013/1/>;
        pav:version            "1";
        void:inDataset         <http://vocab.nerc.ac.uk/.well-known/void>;
        owl:deprecated         "false";
        owl:versionInfo        "1";
        skos:altLabel          "Climate change";
        skos:definition        "The variation in the Earth's global climate or in regional climates over time. It describes changes in the variability over time scales ranging from decades to millions of years. These changes may come from processes internal to the Earth, be driven by external forces (e.g. variations in sunlight intensity) or, most recently, be caused by human activities."@en;
        skos:notation          "SDN:C34::MRAT0013";
        skos:note              "accepted"@en;
        skos:prefLabel         "Climate change"@en .

<http://vocab.nerc.ac.uk/collection/C34/current/MRAT0009/>
        rdf:type               skos:Concept;
        dce:identifier         "SDN:C34::MRAT0009";
        dc:date                "2007-06-29 16:19:24.0";
        dc:identifier          "SDN:C34::MRAT0009";
        pav:authoredOn         "2007-06-29 16:19:24.0";
        pav:hasCurrentVersion  <http://vocab.nerc.ac.uk/collection/C34/current/MRAT0009/1/>;
        pav:version            "1";
        void:inDataset         <http://vocab.nerc.ac.uk/.well-known/void>;
        owl:deprecated         "false";
        owl:versionInfo        "1";
        skos:altLabel          "Organic enrichment";
        skos:definition        "The enrichment of carbon based compounds above natural levels"@en;
        skos:notation          "SDN:C34::MRAT0009";
        skos:note              "accepted"@en;
        skos:prefLabel         "Organic enrichment"@en .

<http://vocab.nerc.ac.uk/collection/C34/current/MRAT0016/>
        rdf:type               skos:Concept;
        dce:identifier         "SDN:C34::MRAT0016";
        dc:date                "2011-08-26 10:26:06.0";
        dc:identifier          "SDN:C34::MRAT0016";
        pav:authoredOn         "2011-08-26 10:26:06.0";
        pav:hasCurrentVersion  <http://vocab.nerc.ac.uk/collection/C34/current/MRAT0016/2/>;
        pav:hasVersion         <http://vocab.nerc.ac.uk/collection/C34/current/MRAT0016/1/>;
        pav:version            "2";
        void:inDataset         <http://vocab.nerc.ac.uk/.well-known/void>;
        owl:deprecated         "false";
        owl:versionInfo        "2";
        skos:altLabel          "Inapplicable";
        skos:definition        "There is no appropriate value"@en;
        skos:notation          "SDN:C34::MRAT0016";
        skos:note              "accepted"@en;
        skos:prefLabel         "inapplicable"@en .

<http://vocab.nerc.ac.uk/collection/C34/current/MRAT0011/>
        rdf:type               skos:Concept;
        dce:identifier         "SDN:C34::MRAT0011";
        dc:date                "2007-06-29 16:19:24.0";
        dc:identifier          "SDN:C34::MRAT0011";
        pav:authoredOn         "2007-06-29 16:19:24.0";
        pav:hasCurrentVersion  <http://vocab.nerc.ac.uk/collection/C34/current/MRAT0011/1/>;
        pav:version            "1";
        void:inDataset         <http://vocab.nerc.ac.uk/.well-known/void>;
        owl:deprecated         "false";
        owl:versionInfo        "1";
        skos:altLabel          "Alien species";
        skos:definition        "The introduction of organisms that are not indigenous to a given place or area and instead have been accidentally or deliberately transported to this new location by human activity."@en;
        skos:notation          "SDN:C34::MRAT0011";
        skos:note              "accepted"@en;
        skos:prefLabel         "Alien species"@en .

<http://vocab.nerc.ac.uk/collection/C34/current/MRAT0021/>
        rdf:type               skos:Concept;
        dce:identifier         "SDN:C34::MRAT0021";
        dc:date                "2007-12-05 16:07:38.0";
        dc:identifier          "SDN:C34::MRAT0021";
        pav:authoredOn         "2007-12-05 16:07:38.0";
        pav:hasCurrentVersion  <http://vocab.nerc.ac.uk/collection/C34/current/MRAT0021/1/>;
        pav:version            "1";
        void:inDataset         <http://vocab.nerc.ac.uk/.well-known/void>;
        owl:deprecated         "false";
        owl:versionInfo        "1";
        skos:altLabel          "Navigation";
        skos:definition        "Physical effects on the water column or seabed caused by shipping, boating and anchoring."@en;
        skos:notation          "SDN:C34::MRAT0021";
        skos:note              "accepted"@en;
        skos:prefLabel         "Navigation"@en .

<http://vocab.nerc.ac.uk/collection/C34/current/MRAT0020/>
        rdf:type               skos:Concept;
        dce:identifier         "SDN:C34::MRAT0020";
        dc:date                "2007-12-05 16:04:24.0";
        dc:identifier          "SDN:C34::MRAT0020";
        pav:authoredOn         "2007-12-05 16:04:24.0";
        pav:hasCurrentVersion  <http://vocab.nerc.ac.uk/collection/C34/current/MRAT0020/1/>;
        pav:version            "1";
        void:inDataset         <http://vocab.nerc.ac.uk/.well-known/void>;
        owl:deprecated         "false";
        owl:versionInfo        "1";
        skos:altLabel          "Mariculture";
        skos:definition        "The cultivation of marine organisms in their natural habitats, usually for commercial purposes."@en;
        skos:notation          "SDN:C34::MRAT0020";
        skos:note              "accepted"@en;
        skos:prefLabel         "Mariculture"@en .

<http://vocab.nerc.ac.uk/collection/C34/current/MRAT0001/>
        rdf:type               skos:Concept;
        dce:identifier         "SDN:C34::MRAT0001";
        dc:date                "2007-06-29 16:19:24.0";
        dc:identifier          "SDN:C34::MRAT0001";
        pav:authoredOn         "2007-06-29 16:19:24.0";
        pav:hasCurrentVersion  <http://vocab.nerc.ac.uk/collection/C34/current/MRAT0001/1/>;
        pav:version            "1";
        void:inDataset         <http://vocab.nerc.ac.uk/.well-known/void>;
        owl:deprecated         "false";
        owl:versionInfo        "1";
        skos:altLabel          "Land reclaim";
        skos:definition        "Alteration of the state of the seabed for land use"@en;
        skos:notation          "SDN:C34::MRAT0001";
        skos:note              "accepted"@en;
        skos:prefLabel         "Land reclaim"@en .

<http://vocab.nerc.ac.uk/collection/C34/current/MRAT0006/>
        rdf:type               skos:Concept;
        dce:identifier         "SDN:C34::MRAT0006";
        dc:date                "2007-12-05 16:08:54.0";
        dc:identifier          "SDN:C34::MRAT0006";
        pav:authoredOn         "2007-12-05 16:08:54.0";
        pav:hasCurrentVersion  <http://vocab.nerc.ac.uk/collection/C34/current/MRAT0006/2/>;
        pav:hasVersion         <http://vocab.nerc.ac.uk/collection/C34/current/MRAT0006/1/>;
        pav:version            "2";
        void:inDataset         <http://vocab.nerc.ac.uk/.well-known/void>;
        owl:deprecated         "false";
        owl:versionInfo        "2";
        skos:altLabel          "Shellfish harvesting";
        skos:definition        "The removal of wild shellfish from the environment by humans"@en;
        skos:notation          "SDN:C34::MRAT0006";
        skos:note              "accepted"@en;
        skos:prefLabel         "Shellfish harvesting"@en .

<http://vocab.nerc.ac.uk/collection/C34/current/MRAT0012/>
        rdf:type               skos:Concept;
        dce:identifier         "SDN:C34::MRAT0012";
        dc:date                "2007-06-29 16:19:24.0";
        dc:identifier          "SDN:C34::MRAT0012";
        pav:authoredOn         "2007-06-29 16:19:24.0";
        pav:hasCurrentVersion  <http://vocab.nerc.ac.uk/collection/C34/current/MRAT0012/1/>;
        pav:version            "1";
        void:inDataset         <http://vocab.nerc.ac.uk/.well-known/void>;
        owl:deprecated         "false";
        owl:versionInfo        "1";
        skos:altLabel          "Abstraction and flow regulation";
        skos:definition        "The removal of water from the marine environment, and/or the anthropogenic regulation of flow by barrages, wiers or other permanent structures"@en;
        skos:notation          "SDN:C34::MRAT0012";
        skos:note              "accepted"@en;
        skos:prefLabel         "Abstraction and flow regulation"@en .

<http://vocab.nerc.ac.uk/collection/C34/current/MRAT0008/>
        rdf:type               skos:Concept;
        dce:identifier         "SDN:C34::MRAT0008";
        dc:date                "2007-06-29 16:19:24.0";
        dc:identifier          "SDN:C34::MRAT0008";
        pav:authoredOn         "2007-06-29 16:19:24.0";
        pav:hasCurrentVersion  <http://vocab.nerc.ac.uk/collection/C34/current/MRAT0008/1/>;
        pav:version            "1";
        void:inDataset         <http://vocab.nerc.ac.uk/.well-known/void>;
        owl:deprecated         "false";
        owl:versionInfo        "1";
        skos:altLabel          "Nutrient enrichment";
        skos:definition        "The enrichment of nutrients particularly nitrogen species, phosphate and silicate above natural levels"@en;
        skos:notation          "SDN:C34::MRAT0008";
        skos:note              "accepted"@en;
        skos:prefLabel         "Nutrient enrichment"@en .

<http://vocab.nerc.ac.uk/collection/C34/current/>
        rdf:type                skos:Collection;
        rdfs:comment            "Governance for vocabularies used in the EU SeaDataNet project implemented as consultation between BODC and the members of the SeaDataNet Technical Task Team";
        dc:alternative          "Purpose categories";
        dc:creator              "SeaDataNet";
        dc:date                 "2011-08-27 02:00:05.0";
        dc:description          "Terms used to specify why an activity was undertaken.";
        dc:license              <https://creativecommons.org/licenses/by/4.0/>;
        dc:publisher            "Natural Environment Research Council";
        dc:title                "Activity purpose categories";
        grg:RE_RegisterManager  "British Oceanographic Data Centre";
        grg:RE_RegisterOwner    "SeaDataNet";
        owl:versionInfo         "4";
        skos:altLabel           "Purpose categories";
        skos:member             <http://vocab.nerc.ac.uk/collection/C34/current/MRAT0014/> , <http://vocab.nerc.ac.uk/collection/C34/current/MRAT0022/> , <http://vocab.nerc.ac.uk/collection/C34/current/MRAT0002/> , <http://vocab.nerc.ac.uk/collection/C34/current/MRAT0007/> , <http://vocab.nerc.ac.uk/collection/C34/current/MRAT0017/> , <http://vocab.nerc.ac.uk/collection/C34/current/MRAT0004/> , <http://vocab.nerc.ac.uk/collection/C34/current/MRAT0018/> , <http://vocab.nerc.ac.uk/collection/C34/current/MRAT0005/> , <http://vocab.nerc.ac.uk/collection/C34/current/MRAT0015/> , <http://vocab.nerc.ac.uk/collection/C34/current/MRAT0003/> , <http://vocab.nerc.ac.uk/collection/C34/current/MRAT0019/> , <http://vocab.nerc.ac.uk/collection/C34/current/MRAT0010/> , <http://vocab.nerc.ac.uk/collection/C34/current/MRAT0013/> , <http://vocab.nerc.ac.uk/collection/C34/current/MRAT0009/> , <http://vocab.nerc.ac.uk/collection/C34/current/MRAT0016/> , <http://vocab.nerc.ac.uk/collection/C34/current/MRAT0011/> , <http://vocab.nerc.ac.uk/collection/C34/current/MRAT0021/> , <http://vocab.nerc.ac.uk/collection/C34/current/MRAT0020/> , <http://vocab.nerc.ac.uk/collection/C34/current/MRAT0001/> , <http://vocab.nerc.ac.uk/collection/C34/current/MRAT0006/> , <http://vocab.nerc.ac.uk/collection/C34/current/MRAT0008/> , <http://vocab.nerc.ac.uk/collection/C34/current/MRAT0012/>;
        skos:prefLabel          "Activity purpose categories" .
