PREFIX : <http://def.isotc211.org/iso19139/2005/MD_GeometricObjectTypeCode/>
PREFIX cs: <http://def.isotc211.org/iso19139/2005/MD_GeometricObjectTypeCode>
PREFIX owl: <http://www.w3.org/2002/07/owl#>
PREFIX rdfs: <http://www.w3.org/2000/01/rdf-schema#>
PREFIX schema: <https://schema.org/>
PREFIX skos: <http://www.w3.org/2004/02/skos/core#>
PREFIX xsd: <http://www.w3.org/2001/XMLSchema#>

:MD_GeometricObjectTypeCode_curve
    a skos:Concept ;
    rdfs:isDefinedBy cs: ;
    skos:definition "Name of point or vector objects used to locate zero-, one-, two-, or three-dimensional spatial locations in the dataset"@en ;
    skos:inScheme cs: ;
    skos:prefLabel "curve"@en ;
    skos:topConceptOf cs: ;
.

:MD_GeometricObjectTypeCode_point
    a skos:Concept ;
    rdfs:isDefinedBy cs: ;
    skos:definition "Name of point or vector objects used to locate zero-, one-, two-, or three-dimensional spatial locations in the dataset"@en ;
    skos:inScheme cs: ;
    skos:prefLabel "point"@en ;
    skos:topConceptOf cs: ;
.

:MD_GeometricObjectTypeCode_surface
    a skos:Concept ;
    rdfs:isDefinedBy cs: ;
    skos:definition "Name of point or vector objects used to locate zero-, one-, two-, or three-dimensional spatial locations in the dataset"@en ;
    skos:inScheme cs: ;
    skos:prefLabel "surface"@en ;
    skos:topConceptOf cs: ;
.

<https://kurrawong.ai>
    a schema:Organization ;
    schema:description "KurrawongAI is a small, Australian-based company enabling organisations to take control of their data." ;
    schema:name "KurrawongAI" ;
    schema:url "https://kurrawong.ai"^^xsd:anyURI ;
.

<https://linked.data.gov.au/org/bodc>
    a schema:Organization ;
    owl:sameAs <https://ror.org/03102fn17> ;
    schema:description """The BODC's mission is to 'operate as a world-class data centre in support of UK marine science'.
    
The BODC is an independent self-governing organisation.""" ;
    schema:name "British Oceanographic Data Centre" ;
    schema:url "https://www.bodc.ac.uk"^^xsd:anyURI ;
.

<https://linked.data.gov.au/org/tc211>
    a schema:Organization ;
    schema:description "The International Organization for Standardization's Technical Committee on \"Geographic information/Geomatics\", is charged with standardization in the field of digital geographic information." ;
    schema:name "ISO's Technical Committee 211" ;
    schema:parentOrganization <https://linked.data.gov.au/org/iso> ;
    schema:url "https://www.iso.org/committee/54904.html"^^xsd:anyURI ;
.

cs:
    a skos:ConceptScheme ;
    skos:definition "Name of point or vector objects used to locate zero-, one-, two-, or three-dimensional spatial locations in the dataset"@en ;
    skos:hasTopConcept
        :MD_GeometricObjectTypeCode_curve ,
        :MD_GeometricObjectTypeCode_point ,
        :MD_GeometricObjectTypeCode_surface ;
    skos:historyNote "This SKOS form of this codelist was produces for the British Oceanographic Data Centre's contribution to the FAIR EASE project which involved the establishment of a Semantic Analyser tool that extracted keywords from ISO 19139 XML data and comared them to a knowledge Base" ;
    skos:prefLabel "Geometric Object Type Code"@en ;
    schema:contributor
        <https://kurrawong.ai> ,
        <https://linked.data.gov.au/org/bodc> ;
    schema:creator <https://linked.data.gov.au/org/tc211> ;
    schema:dateCreated "2005"^^xsd:gYear ;
    schema:dateModified "2005"^^xsd:gYear ;
    schema:publisher <https://linked.data.gov.au/org/tc211> ;
.
